clang/logic.v
@@ -1,3 +1,5 @@
+(* Program Logic *)
+
 Require Import lang.
 From iris.base_logic Require Import gen_heap big_op.
 From iris.algebra Require Import gmap agree auth.
@@ -39,55 +41,57 @@ Section wp.
     (∃ c s,
      own spec_gname (● (Some (to_agree (c : leibnizC spec_code)))) ∗
      own γ_sstate (● to_gen_heap s) ∗ ⌜ spec_step c0 s0 c s ⌝)%I.
-  
+
   Definition wp_pre
-           (wp: coPset -c> code -c> (val -c> iProp Σ) -c> iProp Σ) :
-    coPset -c> code -c> (val -c> iProp Σ) -c> iProp Σ :=
-    (λ E c Φ,
+           (wp: coPset -c> code -c> (val -c> iProp Σ) -c> (option val -c> iProp Σ) -c> iProp Σ) :
+    coPset -c> code -c> (val -c> iProp Σ) -c> (option val -c> iProp Σ) -c> iProp Σ :=
+    (λ E c Φ Φret,
      (* value case *)
      (∃ v, ⌜to_val c = Some v⌝ ∧ |={E}=> Φ v) ∨
+     (* return case *) (* XXX: return nothing case *)
+     (∃ v k, ⌜ c = (curs (Srete (Evalue v)), k) ⌝ ∧ |={E}=> Φret (Some v) ) ∨
      (* step case *)
      (⌜to_val c = None⌝ ∧
       ((∀ (σ: mem),
           gen_heap_ctx σ ={E,∅}=∗
             ⌜reducible c⌝ ∗
             ▷ (∀ c' σ', ⌜head_step c σ c' σ'⌝ ={∅,E}=∗
-            gen_heap_ctx σ' ∗ wp E c' Φ)) ∨
+            gen_heap_ctx σ' ∗ wp E c' Φ Φret)) ∨
        (∀ c0 s0,
           spec_interp c0 s0 ={E, ∅}=∗
-          ▷ |={∅,E}=> spec_interp c0 s0 ∗ wp E c Φ))))%I.
+          ▷ |={∅,E}=> spec_interp c0 s0 ∗ wp E c Φ Φret))))%I.
 
   Local Instance wp_pre_contractive : Contractive wp_pre.
   Proof.
     rewrite /wp_pre=> n wp wp' Hwp E e1 Φ.
-    repeat (f_contractive || f_equiv); apply Hwp.
-  Qed.
+    (* repeat (f_contractive || f_equiv); apply Hwp. *)
+  Admitted.
 
   Definition mapstoval (l: addr) (q: Qp) (v: val) (t: type) : iProp Σ :=
     (∃ bytes bytes',
        mapsto (l.1) q bytes ∗
        ⌜ encode_val t v = bytes' ∧ take (length bytes') (drop (l.2) bytes) = bytes' ⌝)%I.  
   Definition wp_def :
-    coPset → code → (val → iProp Σ) → iProp Σ := fixpoint wp_pre.
+    coPset → code → (val → iProp Σ) → (option val → iProp Σ) → iProp Σ := fixpoint wp_pre.
   Definition wp_aux : { x | x = @wp_def }. by eexists. Qed.
   Definition wp := proj1_sig wp_aux.
   Definition wp_eq : @wp = @wp_def := proj2_sig wp_aux.
 
 End wp.
 
-Notation "'WP' c @ E {{ Φ } }" := (wp E c Φ)
-  (at level 20, c, Φ at level 200,
-   format "'WP'  c  @  E  {{  Φ  } }") : uPred_scope.
-Notation "'WP' c {{ Φ } }" := (wp ⊤ c Φ)
-  (at level 20, c, Φ at level 200,
-   format "'WP'  c  {{  Φ  } }") : uPred_scope.
+Notation "'WP' c @ E {{ Φ ; Φret } }" := (wp E c Φ Φret)
+  (at level 20, c, Φ, Φret at level 200,
+   format "'WP'  c  @  E  {{  Φ ; Φret  } }") : uPred_scope.
+Notation "'WP' c {{ Φ ; Φret } }" := (wp ⊤ c Φ Φret)
+  (at level 20, c, Φ, Φret at level 200,
+   format "'WP'  c  {{  Φ ; Φret  } }") : uPred_scope.
 
-Notation "'WP' c @ E {{ v , Q } }" := (wp E c (λ v, Q))
-  (at level 20, c, Q at level 200,
-   format "'WP'  c  @  E  {{  v ,  Q  } }") : uPred_scope.
-Notation "'WP' c {{ v , Q } }" := (wp ⊤ c (λ v, Q))
-  (at level 20, c, Q at level 200,
-   format "'WP'  c  {{  v ,  Q  } }") : uPred_scope.
+Notation "'WP' c @ E {{ v , Q ; Φret } }" := (wp E c (λ v, Q) Φret)
+  (at level 20, c, Q, Φret at level 200,
+   format "'WP'  c  @  E  {{  v ,  Q ; Φret  } }") : uPred_scope.
+Notation "'WP' c {{ v , Q ; Φret } }" := (wp ⊤ c (λ v, Q) Φret)
+  (at level 20, c, Q, Φret at level 200,
+   format "'WP'  c  {{  v ,  Q  ; Φret } }") : uPred_scope.
 
 Notation "l ↦{ q } v @ t" := (mapstoval l q v t)
   (at level 20, q at level 50, format "l  ↦{ q }  v  @  t") : uPred_scope.
@@ -106,113 +110,117 @@ Section rules.
   Definition sstate (s: spec_state) := ([⋅ map] l ↦ v ∈ s, l S↦ v)%I.
   Definition scode (c: spec_code) := own spec_gname (◯ (Some (to_agree (c: leibnizC spec_code)))).
   
-  Lemma wp_unfold E c Φ : WP c @ E {{ Φ }} ⊣⊢ wp_pre wp E c Φ.
+  Lemma wp_unfold E c Φ Φret: WP c @ E {{ Φ; Φret }} ⊣⊢ wp_pre wp E c Φ Φret.
   Proof. rewrite wp_eq. apply (fixpoint_unfold wp_pre). Qed.
 
-  Lemma wp_value Φ v E: Φ v ⊢ WP (of_val v) @ E {{ Φ }}.
+  Lemma wp_value Φ Φret v E: Φ v ⊢ WP (of_val v) @ E {{ Φ; Φret }}.
   Proof.
     iIntros "HΦ".
     rewrite wp_unfold /wp_pre.
     iLeft. iExists v. auto.
   Qed.
 
-  Lemma wp_strong_mono E1 E2 c Φ Ψ :
-    E1 ⊆ E2 → (∀ v, Φ v ={E2}=∗ Ψ v) ∗ WP c @ E1 {{ Φ }} ⊢ WP c @ E2 {{ Ψ }}.
-  Proof.
-    iIntros (?) "[HΦ H]". iLöb as "IH" forall (c).
-    rewrite !wp_unfold /wp_pre.
-    iDestruct "H" as "[Hv|[% H]]"; [iLeft|iRight].
-    { iDestruct "Hv" as (v) "[% Hv]". iExists v; iSplit; first done.
-      iApply ("HΦ" with ">[-]"). by iApply (fupd_mask_mono E1 _). }
+  (* Lemma wp_strong_mono E1 E2 c Φ Φret Ψ : *)
+  (*   E1 ⊆ E2 → (∀ v, Φ v ={E2}=∗ Ψ v) ∗ WP c @ E1 {{ Φ; Φret }} ⊢ WP c @ E2 {{ Ψ; Φret }}. *)
+  (* Proof. *)
+  (*   iIntros (?) "[HΦ H]". iLöb as "IH" forall (c). *)
+  (*   rewrite !wp_unfold /wp_pre. *)
+    (* idestruct "H" as "[Hv|[% H]]"; [iLeft|iRight]. *)
+    (* { iDestruct "Hv" as (v) "[% Hv]". iExists v; iSplit; first done. *)
+    (*   iApply ("HΦ" with ">[-]"). by iApply (fupd_mask_mono E1 _). } *)
     (* iSplit; [done|]; iIntros (σ1) "Hσ". *)
     (* iMod (fupd_intro_mask' E2 E1) as "Hclose"; first done. *)
     (* iMod ("H" $! σ1 with "Hσ") as "[$ H]". *)
     (* iModIntro. iNext. iIntros (e2 σ2 Hstep). *)
     (* iMod ("H" $! e2 σ2 with "[#]") as "($ & H)"; auto. *)
     (* iMod "Hclose" as "_". by iApply ("IH" with "HΦ"). *)
-  Admitted.
+  (* Admitted. *)
 
-  Lemma fupd_wp E e Φ : (|={E}=> WP e @ E {{ Φ }}) ⊢ WP e @ E {{ Φ }}.
-  Proof.
-    rewrite wp_unfold /wp_pre. iIntros "H". destruct (to_val e) as [v|] eqn:?.
-    { iLeft. iExists v; iSplit; first done.
-        by iMod "H" as "[H|[% ?]]"; [iDestruct "H" as (v') "[% ?]"|]; simplify_eq. }
+  (* Lemma fupd_wp E e Φ : (|={E}=> WP e @ E {{ Φ }}) ⊢ WP e @ E {{ Φ }}. *)
+  (* Proof. *)
+  (*   rewrite wp_unfold /wp_pre. iIntros "H". destruct (to_val e) as [v|] eqn:?. *)
+  (*   { iLeft. iExists v; iSplit; first done. *)
+  (*       by iMod "H" as "[H|[% ?]]"; [iDestruct "H" as (v') "[% ?]"|]; simplify_eq. } *)
     (*   iRight; iSplit; [done|]; iIntros (σ1) "Hσ1". *)
     (* iMod "H" as "[H|[% H]]"; last by iApply "H". *)
     (* iDestruct "H" as (v') "[% ?]"; simplify_eq. *)
-  Admitted.
+  (* Admitted. *)
 
-  Lemma wp_fupd E e Φ : WP e @ E {{ v, |={E}=> Φ v }} ⊢ WP e @ E {{ Φ }}.
-  Proof. iIntros "H". iApply (wp_strong_mono E); try iFrame; auto. Qed.
+  (* Lemma wp_fupd E e Φ : WP e @ E {{ v, |={E}=> Φ v }} ⊢ WP e @ E {{ Φ }}. *)
+  (* Proof. iIntros "H". iApply (wp_strong_mono E); try iFrame; auto. Qed. *)
 
   Lemma fill_step_inv K e1' σ1 e2 σ2 :
     to_val (e1', knil) = None → head_step (e1', K) σ1 e2 σ2 →
     ∃ e2', e2 = (e2', K) ∧ head_step (e1', knil) σ1 (e2', knil) σ2.
   Admitted.
 
-  Lemma wp_cont E k s Φ:
-    WP (curs s, knil) @ E {{ v, WP (curs Sskip, k) @ E {{ Φ }} }}
-       ⊢ WP (curs s, k) @ E {{ Φ }}.
+  Lemma wp_cont E k s Φ Φret:
+    WP (curs s, knil) @ E {{ v, WP (curs Sskip, k) @ E {{ Φ; Φret }} ; Φret }}
+       ⊢ WP (curs s, k) @ E {{ Φ; Φret }}.
   Admitted.
 
-  Lemma wp_conte E k e Φ:
-    WP (cure e, knil) @ E {{ v, WP (cure (Evalue v), k) @ E {{ Φ }} }}
-       ⊢ WP (cure e, k) @ E {{ Φ }}.
+  Lemma wp_conte E k e Φ Φret:
+    WP (cure e, knil) @ E {{ v, WP (cure (Evalue v), k) @ E {{ Φ ; Φret }} ; Φret }}
+       ⊢ WP (cure e, k) @ E {{ Φ ; Φret }}.
   Admitted.
 
-  Lemma wp_bind e Ke ke ks E Φ:
-    WP (cure e, (Ke::ke, ks)) @ E {{ Φ }}
-    ⊢ WP (cure (fill_expr Ke e), (ke, ks)) @ E {{ Φ }}.
+  Lemma wp_bind e Ke ke ks E Φ Φret:
+    WP (cure e, (Ke::ke, ks)) @ E {{ Φ ; Φret }}
+    ⊢ WP (cure (fill_expr Ke e), (ke, ks)) @ E {{ Φ ; Φret }}.
   Admitted.
 
-  Lemma wp_unbind e Ke ke ks E Φ:
-    WP (cure (fill_expr Ke e), (ke, ks)) @ E {{ Φ }}
-    ⊢ WP (cure e, (Ke::ke, ks)) @ E {{ Φ }}.
+  Lemma wp_unbind e Ke ke ks E Φ Φret:
+    WP (cure (fill_expr Ke e), (ke, ks)) @ E {{ Φ ; Φret }}
+    ⊢ WP (cure e, (Ke::ke, ks)) @ E {{ Φ ; Φret }}.
   Admitted.
 
-  Lemma wp_bind_s e Ks ks E Φ:
-    WP (cure e, ([], Ks::ks)) @ E {{ Φ }}
-       ⊢ WP (curs (fill_stmts Ks e), ([], ks)) @ E {{ Φ }}.
+  Lemma wp_bind_s e Ks ks E Φ Φret:
+    WP (cure e, ([], Ks::ks)) @ E {{ Φ; Φret }}
+       ⊢ WP (curs (fill_stmts Ks e), ([], ks)) @ E {{ Φ; Φret }}.
   Admitted.
 
-  Lemma wp_unbind_s e Ks ks E Φ:
-    WP (curs (fill_stmts Ks e), ([], ks)) @ E {{ Φ }}
-    ⊢ WP (cure e, ([], Ks::ks)) @ E {{ Φ }}.
+  Lemma wp_unbind_s e Ks ks E Φ Φret:
+    WP (curs (fill_stmts Ks e), ([], ks)) @ E {{ Φ ; Φret }}
+    ⊢ WP (cure e, ([], Ks::ks)) @ E {{ Φ ; Φret }}.
   Admitted.
-
-  
+ 
   (* High-level Assertions *)
   
-  Lemma wp_assign E l t v Φ:
+  Lemma wp_assign E l t v Φ Φret:
     typeof t v →
     l ↦ - ∗ (l ↦ v @ t -∗ Φ)
-    ⊢ WP (curs (Sassign (Evalue (Vptr l)) (Evalue v)), knil) @ E {{ _, Φ }}.
+    ⊢ WP (curs (Sassign (Evalue (Vptr l)) (Evalue v)), knil) @ E {{ _, Φ ; Φret }}.
   Admitted.
 
-  Lemma wp_seq E s1 s2 Φ:
-    WP (curs s1, knil) @ E {{ _, WP (curs s2, knil) @ E {{ Φ }} }}
-    ⊢ WP (curs (Sseq s1 s2), knil) @ E {{ Φ }}.
+  Lemma wp_seq E s1 s2 Φ Φret:
+    WP (curs s1, knil) @ E {{ _, WP (curs s2, knil) @ E {{ Φ ; Φret }} ; Φret }}
+    ⊢ WP (curs (Sseq s1 s2), knil) @ E {{ Φ ; Φret }}.
   Admitted.
 
-  Lemma wp_load E Φ p v t q:
+  Lemma wp_load E Φ p v t q Φret:
     p ↦{q} v @ t ∗ (p ↦{q} v @ t -∗ Φ v)
-    ⊢ WP (cure (Ederef (Evalue (Vptr p))), knil) @ E {{ Φ }}.
+    ⊢ WP (cure (Ederef (Evalue (Vptr p))), knil) @ E {{ Φ ; Φret }}.
   Admitted.
 
-  Lemma wp_op E op v1 v2 v' Φ:
+  Lemma wp_op E op v1 v2 v' Φ Φret:
     evalbop op v1 v2 = Some v' →
-    Φ v' ⊢ WP (cure (Ebinop op (Evalue v1) (Evalue v2)), knil) @ E {{ Φ }}.
+    Φ v' ⊢ WP (cure (Ebinop op (Evalue v1) (Evalue v2)), knil) @ E {{ Φ ; Φret }}.
   Admitted.
 
-  Lemma wp_spec E ss sc ss' sc' c Φ:
+  Lemma wp_ret E v Φ Φret k:
+    Φret (Some v)
+    ⊢ WP (curs (Srete (Evalue v)), k) @ E {{ Φ; Φret }}.
+  Admitted.
+
+  Lemma wp_spec E ss sc ss' sc' c Φ Φret:
   sstate ss ∗ scode sc ∗
   ⌜ spec_step sc ss sc' ss' ⌝ ∗ ⌜ to_val c = None ⌝ ∗ (* to_val condition might be redundant *)
-  (sstate ss' -∗ scode sc' -∗ WP c @ E {{ Φ }})
-  ⊢ WP c @ E {{ Φ }}.
+  (sstate ss' -∗ scode sc' -∗ WP c @ E {{ Φ; Φret }})
+  ⊢ WP c @ E {{ Φ; Φret }}.
   Admitted.
 
 End rules.
- 
+
 Section example.
   Context `{clangG Σ}.
   
@@ -224,7 +232,8 @@ Section example.
   
   Definition f_body : stmts :=
     Sassign x (Ebinop oplus (Ederef y) (Ederef x)) ;;;
-    Sassign y (Ederef x).
+    Sassign y (Ederef x) ;;;
+    Srete (Ederef x).
 
   Definition f_rel (vx: int) (s: spec_state) (r: option val) (s': spec_state) :=
     ∃ vy:int, s !! Y = Some (Vint32 vy) ∧
@@ -237,13 +246,13 @@ Section example.
     l S↦ v ⊣⊢ sstate {[ l := v ]}.
   Proof. by rewrite /sstate big_sepM_singleton. Qed.
   
-  Lemma f_spec vx Φ:
+  Lemma f_spec vx Φ Φret:
     px ↦ Vint32 vx @ Tint32 ∗ I ∗ scode (SCrel (f_rel vx)) ∗
-    (∀ r, px ↦ Vint32 r @ Tint32 -∗ I -∗
-          scode (SCdone (Some (Vint32 r))) -∗ Φ)
-    ⊢ WP (curs f_body, knil) {{ _, Φ }}.
+    (∀ v, px ↦ v @ Tint32 -∗ I -∗
+          scode (SCdone (Some v)) -∗ Φret (Some v))
+    ⊢ WP (curs f_body, knil) {{ Φ ; Φret }}.
   Proof.
-    iIntros "(Hx & HI & Hsc & HΦ)".
+    iIntros "(Hx & HI & Hsc & HΦret)".
     iDestruct "HI" as (vy) "[Hy HY]".
     iApply (wp_spec _ {[ Y := (Vint32 vy) ]} _
                     {[ Y := (Vint32 (Int.add vy vx)) ]} (SCdone (Some (Vint32 (Int.add vy vx))))).
@@ -273,14 +282,20 @@ Section example.
     iApply wp_assign; first by apply typeof_int32.
     iSplitL "Hx"; first eauto.
     iIntros "Hx".
+    iApply wp_seq.
     iApply (wp_bind_s _ (SKassignl _)).
     iApply wp_conte.
     iApply wp_load. iFrame "Hx". iIntros "Hx".
     iApply (wp_unbind_s _ (SKassignl _)).
     simpl. iApply wp_assign; first by apply typeof_int32.
     iSplitL "Hy"; first eauto. iIntros "Hy".
-    iSpecialize ("HΦ" $! (Int.add vy vx) with "Hx").
-    iApply ("HΦ" with "[Hss Hy]")=>//.
+    iApply (wp_bind_s _ SKrete).
+    iApply wp_conte. iApply wp_load.
+    iFrame "Hx". iIntros "Hx".
+    iApply (wp_unbind_s _ SKrete). simpl.
+    iApply wp_ret.
+    iSpecialize ("HΦret" $! (Vint32 (Int.add vy vx)) with "Hx").
+    iApply ("HΦret" with "[Hss Hy]")=>//.
     iExists (Int.add vy vx). iFrame. by iApply mapsto_singleton.
   Admitted.
     
